\section{Биномиальная формула}
\begin{Def}
Кольцо многочленов от $n$ переменных.
$$(((A[x_1])[x_2])[x_3] \ldots )[x_n]$$
$$(A[x_2])[x_1] = (A[x_1])[x_2]$$
$$x_1 \to x_1$$
$$x_2 \to x_2$$

$$\sum c_{i_1, i_2}x_{1}^{i_1}x_2^{i_2}$$
$A[x_1, \ldots, x_n]$ "--- кольцо многочленов от нескольких переменных.
$$\sum c_{i_1, \ldots, i_n}x_1^{i_1}\ldots x_n^{i_n} $$
\end{Def}

\textbf{Биномиальная формула}: $(x + y)^n = ?$
\textbf{Биномиальные коэффициенты}: $\Choose{n}{k} = \frac{n!}{k!(n - k)!}$

\begin{lemma} 
\begin{enumerate}
\item $\Choose{n}{0} = 1$
\item $\Choose{n}{n} = 1$
\item $\Choose{n}{k} + \Choose{n}{k + 1} = \Choose{n + 1}{k + 1}$
\item $\Choose{n}{k} = \Choose{n}{n - k}$
\end{enumerate}
\end{lemma}
\begin{proof}
\begin{gather*}
\Choose{n}{k} + \Choose{n}{k + 1} = \frac{n!}{k!(n - k)!} + \frac{n!}{(k + 1)!(n - k - 1)!} = \\
= \frac{n!(k + 1) + n!(n - k)}{(k + 1)! \ldots (n - k)!} = \frac{n!(n + 1)}{(k + 1)!(n + 1 - (k + 1))!} = \Choose{n + 1}{k + 1}
\end{gather*}
\end{proof}

\begin{Def}
Треугольник Паскаля:
\[ \begin{array}{c|ccccc}
& 0 & 1 & 2 & 3 & 4 \\
\hline
0 & 1 &   &   &   &   \\
1 & 1 & 1 &   &   &   \\
2 & 1 & 2 & 1 &   &   \\
3 & 1 & 3 & 3 & 1 &   \\
4 & 1 & 4 & 6 & 4 & 1 \\
\end{array} \]
\end{Def}

\begin{theorem}{Биномиальная формула}
\[ (x + y)^k = \sum_{k = 0}^n \Choose{n}{k} x^ky^{n - k} \]
\end{theorem}

\begin{proof}
Индукция по $n$
\begin{enumerate}
\item $n = 0$
\[ 1 = \Choose{0}{0}x^0y^0 \]
\item $n = 1$
\[ x + y = \Choose{1}{0} x^1y^0 + \Choose{1}{1}x^0y^1 \]
\item $n \to n + 1$
\begin{gather*}
(x + y)^{n + 1} = (x + y)^{n}(x + y) = \left(\sum_{k = 0}^{n}\Choose{n}{k}x^ky^{n - k}\right)(x + y) = \sum_{k = 0}^{n}\Choose{n}{k}x^{k + 1}y^{n - k} + \sum_{k = 0}^{n}\Choose{n}{k}x^ky^{n - k + 1} = \\
= \Choose{n}{n}x^{n + 1} + \sum_{k = 0}^{n - 1}\Choose{n}{k}x^{k + 1}y^{n - k} + \sum_{k = 1}^{n}\Choose{n}{k}x^ky^{n - k + 1} + \Choose{n}{0} y^{n + 1} = \\
= \Choose{n + 1}{n + 1}x^{n + 1} + \sum_{k = 1}^{n}\Choose{n}{k - 1}x^{k}y^{n + 1 - k} + \sum_{k = 1}^{n} \Choose{n}{k}x^ky^{n - k + 1} + \Choose{n + 1}{0}y^{n + 1} = \\
= \Choose{n + 1}{n + 1}x^{n + 1} + \sum_{k = 1}^{n}\left(\Choose{n}{k - 1} + \Choose{n}{k}\right) x^{k}y^{n + 1 - k} + \Choose{n + 1}{0}y^{n + 1} = \\
= \sum_{k = 0}^{n + 1} \Choose{n + 1}{k}x^{k}y^{n + 1 - k} \\
\end{gather*}
\end{enumerate}
\end{proof}

\begin{conseq}
\begin{enumerate}
\item \[ \sum_{k = 0}^{n}\Choose{n}{k} = 2^k \]
\item \[ \sum_{\substack{k = 0..n \\ 2  \mid k}} \Choose{n}{k} = 2^{n - 1} \]
\item \[ \sum_{\substack{k = 0..n \\ 2 \nmid k}} \Choose{n}{k} = 2^{n - 1} \]
\end{enumerate}
\end{conseq}