\section{Теорема о дифференцируемости обратной функции}


\begin{theorem}{Производная обратной функции}
$f: (a, b) \to \R,f^{-1}$ ~--- обратная функция.

$f$ ~--- дифф. в точке $x_0 \in (a, b)$

Тогда $(f^{-1})'(f(x_0)) = \frac{1}{f'(x_0)}$

\end{theorem}

\begin{proof}

$$f^{-1} = g$$
$$g(f(x)) = x$$
$$g'(f(x_0))f'(x_0) = 1$$

Нужна дифф. функции g в точке $f(x_0)$

$$f(x) = f(x_0) + f'(x_0)(x - x_0) + \alpha (x)(x - x_0) \text{где $\alpha(x) \to 0$}$$
$$g(f(x)) = g(f(x_0) + f'(x_0)(x - x_0) + \alpha (x)(x - x_0))$$
$$g(y) = g(f(x_0)) + A(y - f(x_0)) + \beta(y)(y - f(x_0))$$
$$g(f(x)) = g(f(x_0)) + A(f(x) - f(x_0)) + \beta(f(x))(f(x) - f(x_0))$$
$$x = x_0 + A(f'(x_0)(x - x_0) + \alpha(x)(x - x_0)) + \beta(f(x))(f'(x_0)(x - x_0) + \alpha(x)(x - x_0))$$
$$A = \frac{1}{f'(x_0)}, o = \frac{\alpha(x)}{f'(x_0)} + \beta(f(x))(f'(x_0 + \alpha(x)))$$
$$\beta(f(x)) = -\frac{\alpha(x)}{f'(x_0)}\frac{1}{f'(x_0) + \alpha(x)}$$
$$\beta(y) = -\frac{\alpha(g(y))}{f'(x_0)}\frac{1}{f'(x_0) + \alpha(g(y))}$$

Надо понять,что $\beta(y) \to 0$ при $y \to f(x_0)$

Если $y \to f(x_0)$, то $g(y) \to g(f(x_0))$

$$\lim_{y \to f(x_0)}\alpha(g(y)) = \lim_{x \to x_0}\alpha(x) = 0$$
\end{proof}

\begin{conseq}
$$(f^{-1})'(y) = \frac{1}{f'(f^{-1}(y_0))}$$

\end{conseq}