\section{Производные элементарных функций}

\begin{align*}
c' &= 0 \\
(x^p)' &= px^{p-1} \\
(a^x)' &= \ln a a^x \\
(\ln x)' &= \frac1x \\
\sin' x &= \cos x \\
\cos' x &= -\sin x \\
\tg' x &= \frac1{\cos^2 x} \\
\ctg' x &= -\frac1{\sin^2 x} \\
\arctg' x &= \frac1{1+x^2} \\
\arcsin' x &= \frac1{\sqrt{1-x^2}} \\
\end{align*}
\begin{proof}
$$\lim_{h\ra 0} \frac{(x+h)^p - x^p}h = \lim_{h\ra 0} \left(\frac{x^p}{x} \frac{\left(\left(1+\frac{h}x\right)^p-1\right)}{\frac{h}x}\right) = x^{p-1}p$$
$$\lim_{h\ra 0} \frac{a^{x+h}-a^x}h = \lim_{h\ra 0} a_x \frac{a^h-1}h = a_x \ln a$$
$$\lim_{h\ra 0} \frac{\ln (x+h) - \ln x}h = \lim_{h\ra 0} \frac{\ln\left(1+\frac{h}x\right)}{\frac{h}x}\frac1x = \frac1x$$
Лооооооооол что такое, Таня? \\
$\sin x = y$
$$\arcsin' y = (\sin^{-1} y)' = \frac1{\cos y} = \frac1{\sqrt{1-x^2}}$$
$\tg x = y$
$$\arctg' y = (\tg^{-1} y)' = \frac1{\cos^2 y} = \frac1{1+x^2}$$
\end{proof}